Simplify proofs related to unique borrows by making borrows respectfull of iff.

theories/lifetime/model/definitions.v
@@ -183,9 +183,9 @@ Section defs.
   Definition idx_bor_own (q : frac) (i : bor_idx) : iProp Σ :=
     own_bor (i.1) (◯ {[ i.2 := (q, to_agree Bor_in) ]}).
   Definition idx_bor (κ : lft) (i : bor_idx) (P : iProp Σ) : iProp Σ :=
-    (lft_incl κ (i.1) ∗ slice borN (i.2) P)%I.
+    (lft_incl κ (i.1) ∗ ∃ P', ▷ □ (P' ↔ P) ∗ slice borN (i.2) P')%I.
   Definition raw_bor (κ : lft) (P : iProp Σ) : iProp Σ :=
-    (∃ s : slice_name, idx_bor_own 1 (κ, s) ∗ slice borN s P)%I.
+    (∃ s : slice_name, idx_bor_own 1 (κ, s) ∗ ∃ P', ▷ □ (P' ↔ P) ∗ slice borN s P')%I.
   Definition bor (κ : lft) (P : iProp Σ) : iProp Σ :=
     (∃ κ', lft_incl κ κ' ∗ raw_bor κ' P)%I.
 End defs.
